\chapter{Ito calculus}

\section{Ito calculus}

\subsection{Product Rule}

\begin{eqnarray}
d(XY) = XdY + YdX +dX dY
\end{eqnarray}

\subsection{Inversion Rule}
If
\begin{eqnarray}
	f &=& \frac{1}{Y} = Y^{-1}
\end{eqnarray}
then
\begin{eqnarray}
	\frac{\partial f}{\partial Y} &=& -Y^{-2} = -\frac{1}{Y^{2}}\\
	\frac{\partial ^{2}f}{\partial Y^{2}} &=& 2Y^{-3} = \frac{2}{Y^{3}}
\end{eqnarray}
and
\begin{eqnarray}
	\nonumber
	df &=& \frac{\partial f}{\partial Y}dY + \frac{1}{2}\frac{\partial^{2}f}{\partial Y^{2}}dY^{2}\\
	&=& -\frac{dY}{Y^{2}} + \frac{dY^{2}}{Y^{3}}
\end{eqnarray}

\subsection{Quotient Rule}
\begin{eqnarray}
d\bigg(\frac{X}{Y}\bigg) &=& \frac{X}{Y}\left[\frac{dX}{X} - \frac{dY}{Y} - \frac{dX}{X}\frac{dY}{Y} + \Bigg(\frac{dY}{Y}\Bigg)^{2}\right]
\end{eqnarray}

\subsection{Ito Isometry}

\subsection{CEV Process}